current version

theories/small_step.v
@@ -1,4 +1,6 @@
-Require Import syntax.
+Require Import syntax sequences.
+Import List.ListNotations.
+Open Scope list.
 
 Definition is_value v :=
     match v with
@@ -8,61 +10,97 @@ Definition is_value v :=
     | _ => False
     end.
 
-Inductive sred: term -> term -> Prop :=
+Inductive sred: term * list value -> term * list value -> Prop :=
   | sred_beta:
-    forall t u v,
-      t.[Value v/] = u ->
-      sred (App (Lam t) (Value v)) u
-  | sred_app_left:
-    forall t1 t2 u,
-      sred t1 t2 ->
-      sred (App t1 u) (App t2 u)
-  | sred_app_right:
-    forall t sigma u1 u2,
-      sred u1 u2 ->
-      sred (App (Value (Closure t sigma)) u1) (App (Value (Closure t sigma)) u2)
+    forall t v sigma sigma',
+      sred
+        (App (Value (Closure t sigma')) (Value v), sigma)
+        (t, v :: sigma')
 
-  | sred_default_conflict:
+  | sred_lam:
+    forall t sigma,
+      sred
+        (Lam t, sigma)
+        (Value (Closure t sigma), sigma)
+
+  | sred_var:
+    forall x v sigma,
+      Some v = List.nth_error sigma x ->
+      sred
+        (Var x, sigma)
+        (Value v, sigma)
+  | sred_app_left:
+    forall t1 t2 u s1 s2,
+      sred (t1, s1) (t2, s2) ->
+      sred
+        (App t1 u, s1)
+        (App t2 u, s2)
+  (* | sred_app_left_conflict:
+      forall t sigma,
+        sred
+          (App (Value (Closure t sigma)) Conflict)
+          Conflict
+  | sred_app_left_empty:
+    forall t sigma,
+      sred
+        (App (Value (Closure t sigma)) Empty)
+        (Empty) *)
+
+  | sred_app_right:
+    forall t sigma u1 u2 s1 s2,
+      sred (u1, s1) (u2, s2) ->
+      sred
+        (App (Value (Closure t sigma)) u1, s1)
+        (App (Value (Closure t sigma)) u2, s2)
+  (* | sred_app_right_conflict:
+    forall u,
+      sred (App Conflict u) Conflict
+  | sred_app_right_empty:
+    forall u,
+      sred (App Empty u) Empty *)
+
+  (* | sred_defaultConflict:
     forall ts ts1 ti ts2 tj ts3 tjust tcons,
-    List.Forall is_value ts ->
-    ti <> Empty ->
-    tj <> Empty ->
-    ts = (ts1 ++ ti::ts2++tj::ts3)%list ->
-    sred (Default ts tjust tcons) Conflict
+      List.Forall is_value ts ->
+      ti <> Empty ->
+      tj <> Empty ->
+      ts = (ts1 ++ ti::ts2++tj::ts3)%list ->
+      sred (Default ts tjust tcons) Conflict
   | sred_DefaultEValue:
     forall ts1 ti ts2 tjust tcons,
-    List.Forall (eq Empty) ts1 ->
-    List.Forall (eq Empty) ts2 ->
-    ti <> Empty ->
-    is_value ti ->
-    sred (Default (ts1++ti::ts2) tjust tcons) ti
+      List.Forall (eq Empty) ts1 ->
+      List.Forall (eq Empty) ts2 ->
+      ti <> Empty ->
+      is_value ti ->
+      sred (Default (ts1++ti::ts2) tjust tcons) ti
  | sred_DefaultE:
     forall ts1 ti ti' ts2 tj tc,
-    sred ti ti' ->
-    (List.Forall is_value ts1) ->
-    sred (Default (ts1++ti::ts2) tj tc) (Default (ts1++ti'::ts2) tj tc)
+      sred ti ti' ->
+      (List.Forall is_value ts1) ->
+      sred (Default (ts1++ti::ts2) tj tc) (Default (ts1++ti'::ts2) tj tc)
   | sred_DefaultJ:
     forall ts tj1 tj2 tc,
-    List.Forall (eq Empty) ts ->
-    sred tj1 tj2 ->
-    sred (Default ts tj1 tc) (Default ts tj2 tc)
+      List.Forall (eq Empty) ts ->
+      sred tj1 tj2 ->
+      sred (Default ts tj1 tc) (Default ts tj2 tc)
   | sred_DefaultJTrue:
     forall ts tc,
-    List.Forall (eq Empty) ts ->
-    sred (Default ts (Value (Bool true)) tc) tc
+      List.Forall (eq Empty) ts ->
+      sred (Default ts (Value (Bool true)) tc) tc
   | sred_DefaultJFalse:
     forall ts tc,
-    List.Forall (eq Empty) ts ->
-    sred (Default ts (Value (Bool false)) tc) Empty
+      List.Forall (eq Empty) ts ->
+      sred (Default ts (Value (Bool false)) tc) Empty
   | sred_DefaultJEmpty:
     forall ts tc,
-    List.Forall (eq Empty) ts ->
-    sred (Default ts Empty tc) Empty
+      List.Forall (eq Empty) ts ->
+      sred (Default ts Empty tc) Empty
   | sred_DefaultJConflict:
     forall ts tc,
-    List.Forall (eq Empty) ts ->
-    sred (Default ts Conflict tc) Empty
+      List.Forall (eq Empty) ts ->
+      sred (Default ts Conflict tc) Empty *)
 .
+
 
 
 Definition subst_of_env sigma :=
